examples/elliptic/arm/assemblerML.sig
@@ -1,0 +1,23 @@
+signature assemblerML =
+sig
+   val register2int   : Data.register -> int
+
+   val num_to_arm     : Arbnum.num -> Data.instruction
+   val arm_to_num     : Data.instruction -> Arbnum.num
+   val arm_to_string  : Arbnum.num option -> bool -> Data.instruction -> string
+   val string_to_arm  : string -> Data.instruction
+   val branch_to_arm  : Data.condition * bool * Arbnum.num ->
+                        Arbnum.num -> Data.instruction
+
+   val encode_arm             : string -> Arbnum.num
+   val decode_arm             : Arbnum.num option -> Arbnum.num -> string
+   val decode_arm_dec         : Arbnum.num option -> string -> string
+   val decode_arm_hex         : Arbnum.num option -> string -> string
+
+   val assembler_to_string    : Arbnum.num option -> Data.assembler ->
+                                string option -> string
+   val parse_arm_buf          : string -> BasicIO.instream -> Lexing.lexbuf ->
+                                Data.assembler list
+   val parse_arm              : string -> Data.assembler list
+   val validate_instruction   : Data.instruction -> Data.instruction
+end
