examples/elliptic/arm/evalML.sml
@@ -1,0 +1,319 @@
+(* interactive use:
+val _ = loadPath := !loadPath @
+          ["/local/scratch/acjf3/hol98/src/theoryML",
+           "/local/scratch/acjf3/hol98/src/portableML"];
+val _ = app load ["ListPair", "Arbnum", "Redblackmap", "armML", "assemblerML"];
+val _ = load "Mosml";
+val _ = load "Random";
+val _ = installPP numML.pp_num;
+val _ = installPP Arbnum.pp_num;
+*)
+
+(* ------------------------------------------------------------------------- *)
+
+fun to_INT_MIN n =
+  let open numML in
+     ("i" ^ Int.toString n, EXP TWO (fromInt (Int.-(n, 1))))
+  end;
+
+fun to_dimword n =
+  let open numML in
+     ("i" ^ Int.toString n, EXP TWO (fromInt n))
+  end;
+
+fun to_dimindex s =
+  if String.sub(s,0) = #"i" then
+    numML.fromString(String.extract(s,1,NONE))
+  else
+    raise fcpML.IndexUndefined;
+
+val index_list = [2, 3, 4, 5, 6, 7, 8, 12, 16, 20, 24, 28, 30, 32, 64];
+
+val dict_INT_MIN =
+  foldl (fn (n, d) => let val (s,m) = to_INT_MIN n in
+           Redblackmap.insert(d,s,m) end)
+    (Redblackmap.mkDict String.compare) index_list;
+
+val dict_dimword =
+  foldl (fn (n, d) => let val (s,m) = to_dimword n in
+           Redblackmap.insert(d,s,m) end)
+    (Redblackmap.mkDict String.compare) index_list;
+
+fun lookup_index f g (fcpML.Tyvar s) = raise fcpML.IndexUndefined
+  | lookup_index f g (fcpML.Tyop (s, l)) =
+      if null l then
+        f s handle _ => raise fcpML.IndexUndefined
+      else if s = "sum" andalso length l = 2 then
+        g (lookup_index f g (hd l)) (lookup_index f g (hd (tl l)))
+      else
+        raise fcpML.IndexUndefined;
+
+val lookup_INT_MIN =
+  lookup_index (fn s => Redblackmap.find(dict_INT_MIN,s)) numML.*;
+
+val lookup_dimword =
+  lookup_index (fn s => Redblackmap.find(dict_dimword,s)) numML.*;
+
+val lookup_dimindex = lookup_index to_dimindex numML.+;
+
+val _ = wordsML.lookup_INT_MIN := lookup_INT_MIN;
+val _ = wordsML.lookup_dimword := lookup_dimword;
+val _ = fcpML.lookup_dimindex := lookup_dimindex;
+
+val _ = fcpML.dimindex (fcpML.Tyop ("i4", []));
+val _ = wordsML.dimword (fcpML.Tyop ("i4", []));
+val _ = wordsML.INT_MIN (fcpML.Tyop ("i4", []));
+
+val Arbnum2num = numML.fromString o Arbnum.toString;
+val num2Arbnum = Arbnum.fromString o numML.toString;
+
+fun fromNum s n = wordsML.fromNum(numML.fromString n, fcpML.Tyop (s, []));
+fun fromHexNum s n = wordsML.fromNum(numML.fromHexString n, fcpML.Tyop (s, []));
+fun fromArbnum s n = wordsML.fromNum(Arbnum2num n, fcpML.Tyop (s, []));
+
+val fromNum2 = (fromNum "i2"): string -> (bool, armML.i2) fcpML.cart;
+val fromNum4 = (fromNum "i4"): string -> (bool, armML.i4) fcpML.cart;
+val fromNum5 = (fromNum "i5"): string -> (bool, armML.i5) fcpML.cart;
+val fromNum8 = (fromNum "i8"): string -> (bool, armML.i8) fcpML.cart;
+val fromNum12 = (fromNum "i12"): string -> (bool, armML.i12) fcpML.cart;
+val fromNum16 = (fromNum "i16"): string -> (bool, armML.i16) fcpML.cart;
+val fromNum24 = (fromHexNum "i24"): string -> (bool, armML.i24) fcpML.cart;
+val fromNum30 = (fromHexNum "i30"): string -> (bool, armML.i30) fcpML.cart;
+val fromNum32 = (fromHexNum "i32"): string -> (bool, armML.i32) fcpML.cart;
+
+val fromArbnum30 =
+  (fromArbnum "i30"): Arbnum.num -> (bool, armML.i30) fcpML.cart;
+
+val fromArbnum32 =
+  (fromArbnum "i32"): Arbnum.num -> (bool, armML.i32) fcpML.cart;
+
+(* ------------------------------------------------------------------------- *)
+
+local
+  fun add1 a = Data.add32 a Arbnum.one;
+  fun div4 a = Arbnum.div(a,Arbnum.fromInt 4);
+  fun mul4 a = Arbnum.*(a,Arbnum.fromInt 4);
+  val start = Arbnum.zero;
+
+  fun mk_links [] dict n = dict
+    | mk_links (h::r) dict n =
+        case h of
+          Data.Code c => mk_links r dict (add1 n)
+        | Data.BranchS b => mk_links r dict (add1 n)
+        | Data.BranchN b => mk_links r dict (add1 n)
+        | Data.Label s =>
+            mk_links r
+             (Redblackmap.insert(dict, s, "0x" ^ Arbnum.toHexString (mul4 n))) n
+        | Data.Mark m => mk_links r dict (div4 m);
+
+  fun mk_link_table code =
+    let val dict = Redblackmap.mkDict String.compare in
+      mk_links code dict start
+    end;
+
+  fun br_to_word32 (cond,link,label) dict n =
+    let val s = assemblerML.assembler_to_string
+                   NONE (Data.BranchS(cond,link,"")) NONE
+        val address = Redblackmap.find(dict, label)
+    in
+      (fromArbnum32 o assemblerML.encode_arm)
+        ("0x" ^ Arbnum.toHexString (mul4 n) ^ ": " ^ s ^ address)
+    end;
+
+  fun is_label (Data.Label s) = true | is_label _ = false;
+
+  fun lcons h [] = [[h]]
+    | lcons h (x::l) = (h::x)::l;
+
+  fun do_link m l [] dict n = ListPair.zip(m, l)
+    | do_link m l (h::r) dict n =
+        case h of
+           Data.Code c =>
+             do_link m
+               (lcons (fromArbnum32 (assemblerML.arm_to_num (assemblerML.validate_instruction c))) l)
+               r dict (add1 n)
+         | Data.BranchS b =>
+             do_link m (lcons (br_to_word32 b dict n) l) r dict (add1 n)
+         | Data.BranchN b =>
+             let val t = fromArbnum32 (assemblerML.arm_to_num (assemblerML.branch_to_arm b (mul4 n))) in
+               do_link m (lcons t l) r dict (add1 n)
+             end
+         | Data.Label s => do_link m l r dict n
+         | Data.Mark mk => let val k = div4 mk in
+               if k = n then
+                 do_link m l r dict n
+               else if null (hd l) then
+                 do_link (k::(tl m)) l r dict k
+               else
+                 do_link (k::m) ([]::l) r dict k
+             end;
+
+  fun do_links code =
+        let val l = do_link [start] [[]] code (mk_link_table code) start in
+          rev (map (fn (a,b) => (a,rev b)) l)
+        end;
+
+  fun assemble_assambler m a = let
+    val l = do_links a
+    val b = map (fn (m,c) => (fromArbnum30 m, c)) l
+  in
+    foldr (fn ((a,c),t) => armML.::- a c t) m b
+  end
+in
+  fun assemble m file = assemble_assambler m (assemblerML.parse_arm file);
+  fun list_assemble m l =
+    let val nll = String.concat (map (fn s => s ^ "\n") l)
+        val c = substring(nll,0,size nll - 1)
+    in
+      assemble_assambler m (assemblerML.parse_arm_buf "" BasicIO.std_in
+        (Lexing.createLexerString c))
+    end;
+  fun assemble1 m t = list_assemble m [t];
+end;
+
+(* ------------------------------------------------------------------------- *)
+
+val exc_mem = list_assemble (fn x => fromNum32 "E6000010")
+  ["0x0: movs pc, #32",
+   "label: b label",
+   "movs pc, r14",
+   "subs pc, r14, #4",
+   "subs pc, r14, #8",
+   "movs pc, r14",
+   "subs pc, r14, #4",
+   "subs pc, r14, #4"];
+
+fun reg armML.r15 = fromNum32 "20"
+  | reg _ = fromNum32 "0";
+
+fun psr armML.CPSR =
+      armML.SET_NZCV (false,(false,(false,false)))
+        (armML.SET_IFMODE false false armML.usr (fromNum32 "0"))
+  | psr _ =
+      armML.SET_NZCV (false,(false,(false,false)))
+        (armML.SET_IFMODE false false armML.usr (fromNum32 "0"));
+
+val state = armML.state_arme (reg,psr,exc_mem,false);
+
+fun done (armML.state_arme (r,p,m,u)) = u;
+
+val count = ref 0;
+
+fun STATE_ARMe printer n s =
+  if n = 0 then s
+  else
+    let val _ = printer s
+        val _ = count := !count + 1
+        val ns = Mosml.time armML.NEXT_ARMe s in
+      if done s then ns else STATE_ARMe printer (n - 1) ns
+    end;
+
+fun printer (armML.state_arme (r,p,m,u)) =
+  let val pc = armML.FETCH_PC r
+      val ireg = m (armML.ADDR30 pc)
+  in
+    print ("0x" ^ (numML.toHexString (wordsML.w2n pc)) ^ ": ");
+    print (assemblerML.decode_arm NONE (num2Arbnum (wordsML.w2n ireg)) ^ "\n")
+  end;
+
+val max = valOf Int.maxInt;
+
+val final = STATE_ARMe printer max state;
+
+(* ------------------------------------------------------------------------- *)
+
+val i2s = Int.toString;
+
+fun hs n = "0x" ^ Arbnum.toHexString n;
+
+local
+  open Arbnum
+  val twoexp32 = pow(two, fromInt 32)
+  fun num2words2 n l =
+    if n = zero then l else
+      let val (q, r) = divmod(n, twoexp32) in
+        num2words2 q ((hs r)::l)
+      end
+  fun words2num2 [] n = n
+    | words2num2 (i::t) n = words2num2 t (fromInt i + (n * twoexp32))
+in
+  fun num2words s = rev (num2words2 s [])
+  fun words2num l = words2num2 (rev l) zero
+end;
+
+fun num2wordsn n s =
+  let val l = num2words s
+      val ll = length l
+  in
+    if n < ll then
+      List.take(l, n)
+    else
+      l @ List.tabulate(n - ll, fn _ => "0x0")
+  end;
+
+fun prefix_hd s [] = [s]
+  | prefix_hd s (h::t) = (s ^ h)::t;
+
+fun random_word l =
+  words2num (Random.rangelist (0, max) (l, Random.newgen()));
+
+(* ------------------------------------------------------------------------- *)
+
+val a = random_word 17;
+val b = random_word 17;
+
+val prog = list_assemble
+  (assemble exc_mem "../code/add.s")
+ (["0x20:\
+   \mov sp, #0xA000",
+   "mov r0, sp",
+   "add r1, r0, #"^i2s(4 * 17),
+   "add r2, r1, #"^i2s(4 * 17),
+   "bl 0x8000"] @
+   (prefix_hd "0xA000: "
+    (num2wordsn 17 a)) @
+    (num2wordsn 17 b));
+
+val final = Mosml.time (STATE_ARMe printer max) (armML.state_arme (reg,psr,prog,false));
+
+(* ------------------------------------------------------------------------- *)
+
+val a = random_word 9;
+val b = random_word 9;
+
+val prog = list_assemble
+  (assemble exc_mem "../code/mul9.s")
+ (["0x20:\
+   \mov sp, #0xA000",
+   "mov r0, sp",
+   "add r1, r0, #"^i2s(4 * 9),
+   "add r2, r1, #"^i2s(4 * 9),
+   "bl 0x8000"] @
+   (prefix_hd "0xA000: "
+    (num2wordsn 9 a)) @
+    (num2wordsn 9 b));
+
+val final = Mosml.time (STATE_ARMe printer max) (armML.state_arme (reg,psr,prog,false));
+
+(* ------------------------------------------------------------------------- *)
+
+val a = random_word 17;
+val b = random_word 17;
+
+val prog = list_assemble
+  (assemble exc_mem "../code/my_mul.s")
+ (["0x20:\
+   \mov sp, #0xA000",
+   "mov r0, sp",
+   "add r1, r0, #"^i2s(4 * 17),
+   "add r2, r1, #"^i2s(4 * 17),
+   "bl 0x8000"] @
+   (prefix_hd "0xA000: "
+    (num2wordsn 17 a)) @
+    (num2wordsn 17 b));
+
+val final = Mosml.time (STATE_ARMe printer max) (armML.state_arme (reg,psr,prog,false));
+
+(* 7.98s, which is 902 times faster and 184 ips *)
+
+(* ------------------------------------------------------------------------- *)
